remove dependency on bytecode
- copy required definitions into bvlScript.sml
- remove BVL's Print instruction
- better treatment of tag shifts in pat->clos and clos->bvl

only partial progress on updating clos_to_bvlScript.sml

new-backend/bvl_jumpScript.sml
@@ -51,7 +51,7 @@ val bEval_JumpList = prove(
   \\ REPEAT STRIP_TAC \\ fs [rich_listTheory.TAKE_LENGTH_APPEND,
        rich_listTheory.DROP_LENGTH_APPEND]
   \\ Cases_on `k < LENGTH ys` \\ fs []
-  \\ fs [bytecodeTheory.bool_to_tag_def]
+  \\ fs [bool_to_val_def,conLangTheory.true_tag_def,conLangTheory.false_tag_def,pat_tag_shift_def]
   \\ IMP_RES_TAC rich_listTheory.EL_APPEND1 \\ fs []
   \\ `k - LENGTH ys < LENGTH zs` by DECIDE_TAC \\ RES_TAC
   \\ `n + LENGTH ys + (k - LENGTH ys) = n + k` by DECIDE_TAC
